Clean/Circomlib/Bitify.lean
@@ -81,6 +81,8 @@ def arbitraryBitLengthCircuit (n : ℕ) : GeneralFormalCircuit (F p) field (fiel
     ∧ (∀ i (_ : i < n), bits[i] = 0 ∨ bits[i] = 1)
     ∧ fieldFromBits bits = input
 
+  localAdds_eq _ _ _ := by sorry
+
   soundness := by
     circuit_proof_start
     simp only [lc_eq] at h_holds
@@ -119,6 +121,8 @@ def circuit (n : ℕ) (hn : 2^n < p) : GeneralFormalCircuit (F p) field (fields 
 
   Spec input output :=
     input.val < 2^n ∧ output = fieldToBits n input
+
+  localAdds_eq _ _ _ := by sorry
 
   soundness := by
     circuit_proof_start [arbitraryBitLengthCircuit]
@@ -190,6 +194,8 @@ def circuit (n : ℕ) : FormalCircuit (F p) (fields n) field where
   Spec input output :=
     output = fieldFromBits input
     ∧ output.val < 2^n
+
+  localAdds_eq _ _ _ := by sorry
 
   soundness := by
     circuit_proof_start
