Clean/Circomlib/CompConstant.lean
@@ -108,6 +108,8 @@ def circuit (c : ℕ) : FormalCircuit (F p) (fields 254) field where
   Spec bits output :=
     output = if fromBits (bits.map ZMod.val) > c then 1 else 0
 
+  localAdds_eq _ _ _ := by sorry
+
   soundness := by
     simp only [circuit_norm, main]
     sorry
