Clean/Circomlib/Mux1.lean
@@ -75,6 +75,8 @@ def circuit (n : ℕ) : FormalCircuit (F p) (Inputs n) (fields n) where
     ∀ i (_ : i < n),
       output[i] = if s = 0 then (c[i]).1 else (c[i]).2
 
+  localAdds_eq _ _ _ := by sorry
+
   soundness := by
     simp only [circuit_norm, main]
     intro offset env input_var input h_input h_assumptions h_output
@@ -189,6 +191,8 @@ def circuit : FormalCircuit (F p) Inputs field where
   Spec input output :=
     let ⟨c, s⟩ := input
     output = if s = 0 then c[0] else c[1]
+
+  localAdds_eq _ _ _ := by sorry
 
   soundness := by
     simp only [circuit_norm, main]
