Clean/Circomlib/Rotate.lean
@@ -33,6 +33,10 @@ def circuit (n r : ℕ) [NeZero n] : FormalCircuit (F p) (fields n) (fields n) w
 
   Spec input output := output = input.rotate r
 
+  localAdds_eq _ _ _ := by
+    simp [main, circuit_norm, Operations.collectAdds]
+    rfl
+
   soundness := by
     circuit_proof_start
     sorry
