Clean/Gadgets/BLAKE3/BLAKE3G.lean
@@ -62,6 +62,7 @@ instance elaborated (a b c d : Fin 16): ElaboratedCircuit (F p) Inputs BLAKE3Sta
 
   localLength_eq _ n := by
     dsimp only [main, circuit_norm, Xor32.circuit, Addition32.circuit, Rotation32.circuit, Rotation32.elaborated]
+  localAdds_eq _ _ _ := by sorry
   output_eq _ _ := by
     dsimp only [main, circuit_norm, Xor32.circuit, Addition32.circuit, Rotation32.circuit, Rotation32.elaborated]
   subcircuitsConsistent _ _ := by
