Clean/Gadgets/Rotation32/Rotation32Bits.lean
@@ -47,6 +47,7 @@ def elaborated (off : Fin 8) : ElaboratedCircuit (F p) U32 U32 where
   output _inputs i0 := output off i0
   localLength_eq _ i0 := by
     simp only [circuit_norm, main, ByteDecomposition.circuit, ByteDecomposition.elaborated]
+  localAdds_eq _ _ _ := by sorry
   output_eq _ _ := by
     simp only [circuit_norm, main, output, ByteDecomposition.circuit, ByteDecomposition.elaborated]
     apply congrArg U32.fromLimbs
